\documentclass[11pt]{scrartcl}

\usepackage[sexy]{evan}
\usepackage[parfill]{parskip}
\usepackage{amsmath}

\title{Sarthak Infinite Sum Problem Solution}

\begin{document}

\begin{problem}
    The Fibonacci Seqence is defined as follows: $F_{0} = 0$, $F_{1} = 1$, and $F_{n} = F_{n - 1} + F_{n - 2}$ for integers $n \geq 2$. The sum
    \[S = \sum_{n = 0}^{\infty} \frac{F_{n}^{2}}{9^{n}}\]
    can be written as $\frac{m}{n}$ where $m$ and $n$ are relatively prime positive integers. Find $m + n$.
\end{problem}

\begin{soln}
    We use Binet's formula to represent each term as
    \begin{align*}
        F_{n}^{2} &= \frac{(\phi^{n} - (1 - \phi)^{n})^{2}}{5} \\
        &= \frac{\phi^{2n} - 2\phi^{n}(1 - \phi)^{n} + (1 - \phi)^{2n}}{5} \\
        &= \frac{\phi^{2n} - 2(\phi - \phi^{2})^{n} + (1 - \phi)^{2n}}{5}
    \end{align*}
    which makes the sum equal to
    \begin{align*}
        S &= \frac{1}{5}\sum_{n = 0}^{\infty} \frac{\phi^{2n} - 2(\phi - \phi^{2})^{n} + (1 - \phi)^{2n}}{9^{n}} \\
        &= \frac{1}{5}\sum_{n = 0}^{\infty} \frac{\phi^{2n}}{9^{n}} - \frac{2}{5}\sum_{n = 0}^{\infty} \frac{(\phi - \phi^{2})^{n}}{9^{n}} + \frac{1}{5}\sum_{n = 0}^{\infty} \frac{(1 - \phi)^{2n}}{9^{n}} \\
        &= \frac{1}{5} \cdot \frac{1}{1 - \frac{\phi^{2}}{9}} - \frac{2}{5} \cdot \frac{1}{1 - \frac{\phi - \phi^{2}}{9}} + \frac{1}{5} \cdot \frac{1}{1 - \frac{(1 - \phi)^{2}}{9}} \\
        &= \frac{1}{5} \cdot \frac{1}{1 - \frac{3 + \sqrt{5}}{18}} - \frac{2}{5} \cdot \frac{1}{1 + \frac{1}{9}} + \frac{1}{5} \cdot \frac{1}{1 - \frac{3 - \sqrt{5}}{18}} \\
        &= \frac{1}{5} \cdot \frac{1}{\frac{15 - \sqrt{5}}{18}} - \frac{2}{5} \cdot \frac{9}{10} + \frac{1}{5} \cdot \frac{1}{\frac{15 + \sqrt{5}}{18}} \\
        &= \frac{\frac{15 + \sqrt{5}}{18}}{\frac{275}{81}} - \frac{9}{25} + \frac{\frac{15 - \sqrt{5}}{18}}{\frac{275}{81}} \\
        &= \frac{30 \cdot 81}{275 \cdot 18} - \frac{9}{25} \\
        &= \frac{54}{110} - \frac{9}{25} \\
        &= \frac{36}{275}.
    \end{align*}
    So, $m + n = 311$.
\end{soln}

\end{document}